theories/pi/Pi_Instance.v
@@ -74,6 +74,14 @@ Inductive sts : proc -> proc -> Prop :=
 
 #[global] Hint Constructors sts:ccs.
 
+#[global] Instance sts_Proper : Proper (cgr ==> cgr ==> iff) sts.
+Proof.
+  intros x1 x2 Hx y1 y2 Hy.
+  split; intros Hst.
+  - eapply sts_cong; eauto. now rewrite Hx.
+  - eapply sts_cong; eauto with cgr.
+Qed.
+
 Hint Rewrite <- cgr_par_assoc : cgr.
 Hint Rewrite <- n_extrusion : cgr.
 Hint Rewrite cgr_scope : cgr.
@@ -325,36 +333,30 @@ auto with cgr. apply transitivity with ((c ! v • 𝟘) ‖ (x ‖ 𝟘)). auto
 eauto with cgr. 
 Qed.  *)
 
-
-(* For the (LTS-transition), the transitable Guards and transitted terms, that performs a Tau ,
-are pretty all the same, up to ≡* *)
-(* Lemma TransitionShapeForTauAndGuard : forall P V, lts P τ V -> 
-exists M, P ≡* (t • V) + M.
+Lemma TransitionShapeForTauAndGuard : forall P V, ((lts P τ V) /\ (exists L, P = (g L))) -> 
+(exists Q M, ((P ≡* ((t • Q) + M))) /\ (V ≡* (Q))).
 Proof.
 intros P V (Transition & guard_witness). 
-dependent induction Transition.
+dependent induction Transition;
+  try (inversion guard_witness as (g & A); inversion A).
   - exists P. exists 𝟘. split. 
     * apply cgr_choice_nil_rev.
     * apply cgr_refl.
-  - inversion guard_witness as (g & impossible_hyp). inversion impossible_hyp.
-  - inversion guard_witness as (g & impossible_hyp). inversion impossible_hyp.
-  - inversion guard_witness as (g & impossible_hyp). inversion impossible_hyp.
-  - inversion guard_witness as (g & impossible_hyp). inversion impossible_hyp.
-  - inversion guard_witness as (g & impossible_hyp). inversion impossible_hyp.
-  - inversion guard_witness as (g & impossible_hyp). inversion impossible_hyp.
-  - inversion guard_witness as (g & impossible_hyp). inversion impossible_hyp.
   - destruct (IHTransition (reflexivity τ)).
-    * exists p1. reflexivity.
-    * destruct H. destruct H.  exists x. 
-      exists (x0 + p2). split; eauto. apply cgr_trans with (((t • x) + x0) + p2).
+    * now exists p1.
+    * destruct H. destruct H. exists x. 
+      exists (x0 + p2). split; eauto.
+      rewrite <- cgr_choice_assoc.
       apply cgr_choice. assumption.
-      apply cgr_choice_assoc. 
   - destruct (IHTransition (reflexivity τ)).
-    * exists p2. reflexivity.
-    * destruct H. destruct H.  exists x. 
-      exists (x0 + p1). split; eauto. apply cgr_trans with (((t • x) + x0) + p1). apply cgr_trans with (p2 + p1). 
-      apply cgr_choice_com. apply cgr_choice. assumption. apply cgr_choice_assoc.
-Qed. *)
+    * now exists p2.
+    * destruct H. destruct H.
+      exists x.
+      eexists (x0 + p1). split; eauto.
+      rewrite <- cgr_choice_assoc.
+      rewrite cgr_choice_com.
+      apply cgr_choice. assumption.
+Qed.
 
   
 Ltac case_shift :=
@@ -893,10 +895,11 @@ induction n.
 - apply sts_res. exact IHn.
 Qed.
 
-Lemma Communication_Under_News: forall p1 q1 n1 n2 m c v P1 P2 G1 G2 R1 R2,
-p1 ≡* νs n1 ((nvars n1 c) ! (nvars n2 v) • P1 + G1 ‖ R1) ->
-q1 ≡* νs m ((nvars m c) ? P2 + G2 ‖ R2) ->
-(p1 ‖ q1) ≡*
+Lemma Communication_Under_News: forall n1 n2 m c v P1 P2 G1 G2 R1 R2,
+( νs n1 ((nvars n1 c) ! (nvars n2 v) • P1 + G1 ‖ R1)
+‖
+νs m ((nvars m c) ? P2 + G2 ‖ R2))
+≡*
 νs n1
   (νs m
   ((nvars (m + n1) c ! nvars (m + n2) v • nvars m P1 + nvars m G1
@@ -906,7 +909,6 @@ G2 ⟨ upn m (Nat.iter n1 shift) ⟩)
 ‖ (R2 ⟨ upn m (Nat.iter n1 shift) ⟩ ‖ nvars m R1))).
 Proof.
 intros.
-rewrite H, H0.
 rewrite n_extrusion.
 rewrite nvars_νs.
 rewrite cgr_par_com.
@@ -965,7 +967,7 @@ Lemma Taus_Implies_Reduction : forall P Q, (lts P τ Q) -> (sts P Q).
 Proof. 
 intros P Q Transition.
 dependent induction Transition.
-- eapply sts_cong. instantiate (1:=  ((t • P) + 𝟘)). apply cgr_choice_nil_rev. eapply sts_tau. reflexivity.
+- rewrite cgr_choice_nil_rev. apply sts_tau.
 - apply sts_recursion.
 - apply sts_ifOne. assumption.
 - apply sts_ifZero. assumption.
@@ -974,1183 +976,81 @@ dependent induction Transition.
     as (P1 & G1 & R1 & n & Hcongr1 & Hcongr1' & _).
   destruct (TransitionShapeForInput q1 q2 c v  Transition2)
     as (P2 & G2 & R2 & m & Hcongr2 & Hcongr2' & _).
-  eapply sts_cong.
-  + apply Communication_Under_News. exact Hcongr1. exact Hcongr2.
-  + repeat eapply sts_nres. eapply sts_par. eapply sts_com.
-  + rewrite Hcongr1', Hcongr2'. apply Communicated_Under_News.
+  rewrite Hcongr1, Hcongr2, Hcongr1', Hcongr2'.
+  rewrite Communication_Under_News.
+  rewrite <- Communicated_Under_News.
+  repeat eapply sts_nres. eapply sts_par. eapply sts_com.
 (* lts_comR *)
 - destruct (TransitionShapeForFreeOutput p1 p2 c v Transition1)
     as (P1 & G1 & R1 & n & Hcongr1 & Hcongr1' & _).
   destruct (TransitionShapeForInput q1 q2 c v  Transition2)
     as (P2 & G2 & R2 & m & Hcongr2 & Hcongr2' & _).
-  eapply sts_cong.
-  + rewrite cgr_par_com.
-    apply Communication_Under_News. exact Hcongr1. exact Hcongr2.
-  + repeat eapply sts_nres. eapply sts_par. eapply sts_com.
-  + rewrite (cgr_par_com q2). rewrite Hcongr1', Hcongr2'.
-    apply Communicated_Under_News.
+  rewrite cgr_par_com, (cgr_par_com q2).
+  rewrite Hcongr1, Hcongr2, Hcongr1', Hcongr2'.
+  rewrite Communication_Under_News.
+  rewrite <- Communicated_Under_News.
+  repeat eapply sts_nres. eapply sts_par. eapply sts_com.
 (* lts_close_l *)
 - destruct (TransitionShapeForBoundOutput p1 p2 c Transition1)
     as (n & P1 & Q1 & G1 & Hcongr1 & Hcongr1').
   destruct (TransitionShapeForInput _ q2 _ 0 Transition2)
     as (P2 & G2 & R2 & m & Hcongr2 & Hcongr2' & _).
-  eapply sts_cong.
-  + rewrite Hcongr1. simpl. rewrite shift_in_nvars.
-    rewrite cgr_scope_rev.
-    rewrite Hcongr2. eapply cgr_res.
-    apply Communication_Under_News. reflexivity. reflexivity.
-  + eapply sts_res. repeat eapply sts_nres. eapply sts_par. eapply sts_com.
-  + rewrite Hcongr1', Hcongr2'. now rewrite Communicated_Under_News.
+  rewrite Hcongr1. simpl. rewrite shift_in_nvars.
+  rewrite cgr_scope_rev.
+  rewrite Hcongr2.
+  rewrite Communication_Under_News.
+  rewrite Hcongr1', Hcongr2'. rewrite <- Communicated_Under_News.
+  apply sts_res. repeat apply sts_nres. eapply sts_par, sts_com.
 (* lts_close_r *)
+- destruct (TransitionShapeForBoundOutput _ _ c Transition1)
+    as (m & P1 & Q1 & G1 & Hcongr1 & Hcongr1').
+  destruct (TransitionShapeForInput _ _ _ 0 Transition2)
+    as (P2 & G2 & R2 & n & Hcongr2 & Hcongr2' & _).
+  rewrite cgr_par_com.
+  rewrite Hcongr1. simpl. rewrite shift_in_nvars.
+  rewrite cgr_scope_rev.
+  rewrite Hcongr2.
+  rewrite Communication_Under_News.
+  rewrite (cgr_par_com p2). rewrite Hcongr1', Hcongr2'.
+  rewrite <- Communicated_Under_News.
+  apply sts_res. repeat apply sts_nres. eapply sts_par, sts_com.
+(* lts_res *)
 - now apply sts_res, IHTransition.
+(* lts_parL *)
 - now apply sts_par, IHTransition.
-- eapply sts_cong.
-  + apply cgr_par_com.
-  + now eapply sts_par, IHTransition.
-  + apply cgr_par_com.
-- destruct (TransitionShapeForTauAndGuard (g p1) q). split. assumption. exists p1. reflexivity.
-  decompose record H.
-  eapply sts_cong. instantiate (1:= ((t • x) + (x0 + p2))).
-  apply transitivity with (g (((t • x) + x0) + p2)). apply cgr_choice. assumption. apply cgr_choice_assoc.
-  instantiate (1:= x). apply sts_tau. symmetry. assumption.
-- destruct (TransitionShapeForTauAndGuard (g p2) q). split. assumption. exists p2. reflexivity.
-  decompose record H. eapply sts_cong. instantiate (1:= ((t • x) + (x0 + p1))).
-  apply transitivity with (g (((t • x) + x0 ) + p1)). apply transitivity with (g (p2 + p1)). apply cgr_choice_com.
-  apply cgr_choice. assumption. apply cgr_choice_assoc. instantiate (1:= x). apply sts_tau.
-  symmetry. assumption.
+(* lts_parR *)
+- rewrite cgr_par_com. rewrite (cgr_par_com p).
+  now eapply sts_par, IHTransition.
+(* lts_choiceL *)
+- destruct (TransitionShapeForTauAndGuard (g p1) q) as (P & G & H1 & H2).
+  + split. assumption. now exists p1.
+  + rewrite H2.
+    (* This (and the same below) should just be a "rewrite H1" but my typeclasses
+       are likely to blame *)
+    eapply sts_Proper. eapply gpr_choice_proper. unfold gpr_cgr. exact H1.
+    unfold gpr_cgr. reflexivity. reflexivity.
+    rewrite cgr_choice_assoc. apply sts_tau.
+(* lts_choiceR *)
+- destruct (TransitionShapeForTauAndGuard (g p2) q) as (P & G & H1 & H2).
+  + split. assumption. now exists p2.
+  + rewrite H2. eapply sts_Proper. rewrite cgr_choice_com.
+    eapply gpr_choice_proper. unfold gpr_cgr. exact H1.
+    unfold gpr_cgr. reflexivity. reflexivity.
+    rewrite cgr_choice_assoc. apply sts_tau.
 Qed.
 
 (* One side of the Harmony Lemma*)
 Lemma TausAndCong_Implies_Reduction: forall P Q, (lts_then_sc P τ Q) -> (sts P Q).
 Proof.
 intros P Q H.
-apply Congruence_Simplicity with τ. exact Taus_Implies_Reduction. exact H.
+apply Congruence_Simplicity with τ.
+- exact Taus_Implies_Reduction.
+- exact H.
 Qed.
 
-Theorem HarmonyLemmaForCCSWithValuePassing : forall P Q, (lts_then_sc P τ Q) <-> (sts P Q).
+Theorem HarmonyLemma : forall P Q, (lts_then_sc P τ Q) <-> (sts P Q).
 Proof.
 intros. split.
 * apply TausAndCong_Implies_Reduction.
 * apply Reduction_Implies_TausAndCong.
 Qed.
-
-
-
-
-(*
-(*The next work is for making 'bvar' always relates to an input*) 
-
-(* Definition for Well Abstracted bvariable *)
-Inductive Well_Defined_Data : nat -> Data -> Prop :=
-| bvar_is_defined_up_to_k: forall k x, (x < k) -> Well_Defined_Data k (bvar x)
-| cst_is_always_defined : forall k v, Well_Defined_Data k (cst v).
-
-Inductive Well_Defined_Condition : nat -> Equation Data -> Prop :=
-| tt_is_WD : forall k, Well_Defined_Condition k tt
-| ff_is_WD : forall k, Well_Defined_Condition k ff
-| Inequality_is_WD : forall k x y, Well_Defined_Data k x -> Well_Defined_Data k y -> Well_Defined_Condition k (x ⩽ y)
-| Or_is_WD : forall k e e', Well_Defined_Condition k e -> Well_Defined_Condition k e' -> Well_Defined_Condition k (e ∨ e')
-| Not_is_WD : forall k e, Well_Defined_Condition k e -> Well_Defined_Condition k (non e).
-
-(* the 'bvar' always relates to a input *)
-Inductive Well_Defined_Input_in : nat -> proc -> Prop :=
-| WD_par : forall k p1 p2, Well_Defined_Input_in k p1 -> Well_Defined_Input_in k p2 
-                -> Well_Defined_Input_in k (p1 ‖ p2)
-| WD_var : forall k i, Well_Defined_Input_in k (pr_var i)
-| WD_rec : forall k x p1, Well_Defined_Input_in k p1 -> Well_Defined_Input_in k (rec x • p1)
-| WD_if_then_else : forall k p1 p2 C, Well_Defined_Condition k C -> Well_Defined_Input_in k p1 
-                    -> Well_Defined_Input_in k p2 
-                        -> Well_Defined_Input_in k (If C Then p1 Else p2)
-| WD_success : forall k, Well_Defined_Input_in k (①)
-| WD_nil : forall k, Well_Defined_Input_in k (𝟘)
-| WD_input : forall k c p, Well_Defined_Input_in (S k) p
-                  -> Well_Defined_Input_in k (c ? p)
-| WD_output : forall k c v, Well_Defined_Data k v 
-                  -> Well_Defined_Input_in k (c ! v • 𝟘)
-| WD_tau : forall k p,  Well_Defined_Input_in k p -> Well_Defined_Input_in k (t • p)
-| WD_choice : forall k p1 p2,  Well_Defined_Input_in k (g p1) ->  Well_Defined_Input_in k (g p2) 
-              ->  Well_Defined_Input_in k (p1 + p2).
-
-#[global] Hint Constructors Well_Defined_Input_in:ccs.
-
-Lemma Inequation_k_data : forall k d, Well_Defined_Data k d -> Well_Defined_Data (S k) d.
-Proof.
-intros. dependent destruction d. constructor. dependent destruction H. constructor. auto with arith.
-Qed.
-
-Lemma Inequation_k_equation : forall k c, Well_Defined_Condition k c -> Well_Defined_Condition (S k) c.
-Proof.
-intros. dependent induction c.
-* constructor.
-* constructor.
-* destruct a; destruct a0.
-  - constructor; constructor.
-  - dependent destruction H. constructor. constructor. apply Inequation_k_data. assumption.
-  - dependent destruction H. constructor. apply Inequation_k_data. assumption. constructor. 
-  - dependent destruction H. constructor; apply Inequation_k_data; assumption.
-* dependent destruction H. constructor. apply IHc1. assumption. apply IHc2. assumption.
-* dependent destruction H. constructor. apply IHc. assumption.
-Qed.
-
-Lemma Inequation_k_proc : forall k p, Well_Defined_Input_in k p -> Well_Defined_Input_in (S k) p.
-Proof.
-intros. revert H. revert k.
-induction p as (p & Hp) using
-    (well_founded_induction (wf_inverse_image _ nat _ size Nat.lt_wf_0)).
-destruct p.
-- intros. dependent destruction H. constructor; apply Hp; simpl; auto with arith; assumption.
-- intros. constructor.
-- intros. constructor. apply Hp. simpl; auto with arith. dependent destruction H. assumption.
-- intros. dependent destruction H. constructor. 
-  ** apply Inequation_k_equation. assumption.
-  ** apply Hp. simpl; auto with arith. assumption.
-  ** apply Hp. simpl; auto with arith. assumption.
-- intros. constructor. dependent destruction H. apply Inequation_k_data. assumption.
-- destruct g0.
-  ** intros. constructor.
-  ** intros. constructor.
-  ** intros. constructor. apply Hp. simpl; auto with arith. dependent destruction H. assumption.
-  ** intros. constructor. apply Hp. simpl; auto with arith. dependent destruction H. assumption.
-  ** intros. dependent destruction H. constructor.
-    -- apply Hp. simpl; auto with arith. assumption.
-    -- apply Hp. simpl; auto with arith. assumption.
-Qed.
-
-
-Lemma Congruence_step_Respects_WD_k : forall p q k, Well_Defined_Input_in k p -> p ≡ q -> Well_Defined_Input_in k q. 
-Proof.
-intros. revert H. revert k. dependent induction H0 ; intros.
-* auto.
-* dependent destruction H; auto.
-* constructor; auto. constructor.
-* dependent destruction H;constructor; auto.
-* dependent destruction H. dependent destruction H. constructor. auto. constructor;auto.
-* dependent destruction H. dependent destruction H0. constructor;auto. constructor; auto.
-* dependent destruction H; auto.
-* constructor; auto. constructor.
-* dependent destruction H. constructor; auto. 
-* dependent destruction H. dependent destruction H. constructor; auto. constructor; auto.
-* dependent destruction H. dependent destruction H0. constructor; auto. constructor; auto.
-* dependent destruction H. constructor. apply IHcgr_step. auto.
-* dependent destruction H. constructor. apply IHcgr_step. auto.
-* constructor. dependent destruction H. apply IHcgr_step. auto.
-* dependent destruction H. constructor; auto.
-* dependent destruction H. constructor; auto.
-* dependent destruction H. constructor; auto.
-* dependent destruction H. constructor; auto.
-Qed.
-
-Lemma Congruence_Respects_WD_k : forall p q k, Well_Defined_Input_in k p -> p ≡* q -> Well_Defined_Input_in k q. 
-Proof.
-intros. dependent induction H0.
-- apply Congruence_step_Respects_WD_k with x; auto.
-- eauto.
-Qed.
-
-Lemma Congruence_Respects_WD : forall p q, Well_Defined_Input_in 0 p -> p ≡* q -> Well_Defined_Input_in 0 q.
-Proof.
-intros. eapply Congruence_Respects_WD_k; eauto.
-Qed.
-
-Lemma NotK : forall n k,  n < S k -> n ≠ k -> n < k.
-Proof.
-intros. assert (n ≤ k). auto with arith. destruct H1. exfalso. apply H0. reflexivity. auto with arith.
-Qed.
-
-Lemma ForData : forall k v d, Well_Defined_Data (S k) d -> Well_Defined_Data k (subst_Data k (cst v) d).
-Proof.
-intros. revert H. revert v. revert k. dependent induction d.
-* intros. simpl. constructor.
-* intros. simpl. destruct (decide (n = k )).
-  - constructor. 
-  - dependent destruction H. constructor. apply NotK; assumption.
-Qed.
-
-Lemma ForEquation : forall k v e, Well_Defined_Condition (S k) e 
-                -> Well_Defined_Condition k (subst_in_Equation k (cst v) e).
-Proof.
-intros. revert H. revert v. revert k. 
-- dependent induction e. 
--- intros. simpl. constructor.
--- intros. simpl. constructor.
--- dependent induction a; dependent induction a0.
-  * intros. simpl. constructor; constructor.
-  * intros. simpl. destruct (decide (n = k)).
-    ** constructor; constructor.
-    ** constructor. constructor. dependent destruction H. dependent destruction H0. constructor. apply NotK; assumption.
-  * intros. simpl. constructor; try constructor. destruct (decide (n = k)). constructor. dependent destruction H.
-    dependent destruction H. constructor. apply NotK; assumption.
-  * intros. simpl. constructor.
-    ** destruct (decide (n = k)); try constructor. dependent destruction H. dependent destruction H. 
-    apply NotK; assumption.
-    ** destruct (decide (n0 = k)); try constructor. dependent destruction H. dependent destruction H0. 
-    apply NotK; assumption.
--- intros. dependent destruction H. simpl. constructor. apply IHe1. assumption. apply IHe2. assumption.
--- intros. dependent destruction H. simpl. constructor. apply IHe. assumption.
-Qed.
-
-Lemma WD_and_subst_rec : forall k p v, Well_Defined_Input_in (S k) p -> Well_Defined_Input_in k (subst_in_proc k (cst v) p).
-Proof.
-intros. revert v. revert H. revert k.
-induction p as (p & Hp) using
-    (well_founded_induction (wf_inverse_image _ nat _ size Nat.lt_wf_0)).
-destruct p.
-* intros. dependent destruction H. simpl. constructor. 
-  - apply Hp. simpl. auto with arith. assumption.
-  - apply Hp. simpl. auto with arith. assumption.
-* intros. simpl. constructor.
-* intros. simpl. dependent destruction H. constructor. apply Hp. simpl. auto with arith. assumption.
-* intros. simpl. dependent destruction H. constructor.
-  - apply ForEquation. assumption.
-  - apply Hp. simpl. auto with arith. assumption.
-  - apply Hp. simpl. auto with arith. assumption.
-* intros. simpl. dependent destruction H. constructor. apply ForData. assumption.
-* destruct g0.
-  - intros. simpl. constructor.
-  - intros. simpl. constructor.
-  - intros. simpl. constructor. apply Hp. simpl. auto. dependent destruction H. assumption.
-  - intros. simpl. constructor. apply Hp. simpl. auto. dependent destruction H. assumption.
-  - intros. simpl. dependent destruction H. constructor.
-    -- assert (Well_Defined_Input_in k (subst_in_proc k v (g0_1))). apply Hp.
-      simpl.  auto with arith. assumption. assumption.
-    -- assert (Well_Defined_Input_in k (subst_in_proc k v (g0_2))). apply Hp.
-      simpl.  auto with arith. assumption. assumption.
-Qed.
-
-Lemma WD_data_and_NewVar : forall d k i, Well_Defined_Data (k + i) d 
-                          -> Well_Defined_Data (S (k + i)) (NewVar_in_Data i d).
-Proof.
-dependent induction d; intros.
-- simpl. constructor.
-- simpl. destruct (decide (i < S n)).
-  * constructor. simpl. dependent destruction H. auto with arith.
-  * constructor. dependent destruction H. apply transitivity with i.
-    apply Nat.nlt_succ_r. assumption.
-    auto with arith. 
-Qed.
-
-Lemma WD_eq_and_NewVar : forall e k i, Well_Defined_Condition (k + i) e 
-                          -> Well_Defined_Condition (S (k + i)) (NewVar_in_Equation i e).
-Proof.
-intro. dependent induction e; intros; simpl. 
-* constructor.
-* constructor.
-* dependent destruction H.  constructor; apply WD_data_and_NewVar ; assumption.
-* dependent destruction H. constructor. 
-  - apply IHe1. assumption.
-  - apply IHe2. assumption.
-* dependent destruction H. constructor. apply IHe. assumption.
-Qed.
-
-Lemma WD_and_NewVar : forall k i p, Well_Defined_Input_in (k + i) p -> Well_Defined_Input_in ((S k) + i) (NewVar i p).
-Proof.
-intros. revert H. revert k i.
-induction p as (p & Hp) using
-    (well_founded_induction (wf_inverse_image _ nat _ size Nat.lt_wf_0)).
-destruct p; intros; simpl.
-* dependent destruction H. constructor.
-   - apply Hp. simpl. auto with arith. assumption.
-   - apply Hp. simpl. auto with arith. assumption.
-* constructor.
-* constructor. dependent destruction H. apply Hp. simpl. auto with arith. assumption.
-* dependent destruction H. constructor. apply  WD_eq_and_NewVar. assumption.
-   - apply Hp. simpl. auto with arith. assumption.
-   - apply Hp. simpl. auto with arith. assumption.
-* constructor. dependent destruction H. apply WD_data_and_NewVar. assumption.
-* destruct g0; intros; simpl.
-  - constructor.
-  - constructor.
-  - dependent destruction H. constructor. 
-    assert (S (S (k + i)) = (S k + S i)%nat). simpl. auto with arith.
-    rewrite H0. apply Hp. simpl. auto with arith. assert ((k + S i)%nat = S (k + i)).  auto with arith. rewrite H1. assumption.
-  - constructor. apply Hp. simpl. auto. dependent destruction H. assumption.
-  - dependent destruction H. constructor.
-    -- assert (S (k + i) = (S k + i)%nat). auto with arith. rewrite H1.
-       assert (Well_Defined_Input_in (S k + i) (NewVar i (g g0_1))).
-       apply Hp. simpl. auto with arith. assumption. assumption.
-    -- assert (S (k + i) = (S k + i)%nat). auto with arith. rewrite H1.
-       assert (Well_Defined_Input_in (S k + i) (NewVar i (g g0_2))).
-       apply Hp. simpl. auto with arith. assumption. assumption.
-Qed.
-
-Lemma ForRecursionSanity : forall p' p x k, Well_Defined_Input_in k p' -> Well_Defined_Input_in k p 
-            -> Well_Defined_Input_in k (pr_subst x p' p).
-Proof.
-intros. revert H. revert H0. revert k. revert x. revert p.
-induction p' as (p' & Hp) using
-    (well_founded_induction (wf_inverse_image _ nat _ size Nat.lt_wf_0)).
-destruct p'.
-* intros. simpl. constructor. 
-  ** apply Hp. simpl. auto with arith. assumption. dependent destruction H. assumption.
-  ** apply Hp. simpl. auto with arith. assumption. dependent destruction H. assumption.
-* intros. simpl. destruct (decide (x = n)). assumption. assumption.
-* intros. simpl. destruct (decide (x=n)). 
-  ** dependent destruction H. assumption.
-  ** constructor. apply Hp. simpl; auto with arith. assumption. dependent destruction H. assumption.
-* intros. simpl. dependent destruction H. constructor.
-  ** assumption.
-  ** apply Hp. simpl; auto with arith. assumption. assumption.
-  ** apply Hp. simpl; auto with arith. assumption. assumption.
-* intros. simpl. assumption.
-* destruct g0. 
-  ** intros. simpl. constructor.
-  ** intros. simpl. constructor.
-  ** intros. simpl. constructor. dependent destruction H. apply Hp. 
-    - simpl;auto with arith.
-    - assert ((S k) = ((S k) + 0)%nat). auto with arith. rewrite H1. apply (WD_and_NewVar k 0 p0).
-      assert (k = (k + 0)%nat). auto with arith. rewrite <-H2. assumption. 
-    - assumption.
-  ** intros. simpl. constructor. apply Hp.
-    - simpl; auto with arith.
-    - assumption.
-    - dependent destruction H. assumption.
-  ** intros. simpl. dependent destruction H. constructor.
-    - assert (Well_Defined_Input_in k (pr_subst x (g g0_1) p)). apply Hp. simpl; auto with arith. assumption.
-      assumption. assumption.
-    - assert (Well_Defined_Input_in k (pr_subst x (g g0_2) p)). apply Hp. simpl; auto with arith. assumption.
-      assumption. assumption.
-Qed.
-
-Lemma RecursionOverReduction_is_WD : forall k x p, Well_Defined_Input_in k (rec x • p) 
-          -> Well_Defined_Input_in k (pr_subst x p (rec x • p)).
-Proof.
-intros. apply ForRecursionSanity. dependent destruction H. assumption. assumption.
-Qed.
-
-Lemma Well_Def_Data_Is_a_value : forall d, Well_Defined_Data 0 d <-> exists v, d = cst v.
-Proof.
-intros. split. 
-- intro. dependent destruction H. exfalso. dependent induction H. exists v. reflexivity.
-- intros. destruct H. subst. constructor.
-Qed.
-
-Lemma STS_Respects_WD : forall p q, Well_Defined_Input_in 0 p -> sts p q -> Well_Defined_Input_in 0 q.
-Proof.
-intros. revert H. rename H0 into Reduction. dependent induction Reduction.
-* intros. constructor.
-  - constructor.
-  - dependent destruction H. dependent destruction H0. dependent destruction H0_. 
-    dependent destruction H. apply Well_Def_Data_Is_a_value in H. destruct H. subst.  apply WD_and_subst_rec. assumption. 
-* intros. dependent destruction H. dependent destruction H. assumption.
-* intros. dependent destruction H. apply RecursionOverReduction_is_WD. constructor. assumption.
-* intros. dependent destruction H0. assumption.
-* intros. dependent destruction H0. assumption.
-* intros. dependent destruction H. constructor. apply IHReduction. assumption. assumption.
-* intros. apply Congruence_Respects_WD with q2. apply IHReduction. apply Congruence_Respects_WD with p1. 
-  assumption. assumption. assumption.
-Qed.
-
-Inductive Well_Defined_Action: (Act TypeOfActions) -> Prop :=
-| ActionOuput_with_value_is_always_defined : forall c v, Well_Defined_Action (ActOut  (c ⋉ (cst v)))
-| ActionInput_with_value_is_always_defined : forall c v, Well_Defined_Action (ActIn  (c ⋉ (cst v)))
-| Tau_is_always_defined : Well_Defined_Action (τ).
-
-Lemma Output_are_good : forall p1 p2 c d, Well_Defined_Input_in 0 p1 -> lts p1 (ActOut (c ⋉ d)) p2 
-      -> exists v, d = cst v.
-Proof.
-intros. dependent induction H0. dependent destruction H. apply Well_Def_Data_Is_a_value in H. destruct H.
-subst. exists x. reflexivity.
-- dependent destruction H. eapply IHlts with c. assumption. reflexivity.
-- dependent destruction H. eapply IHlts with c. assumption. reflexivity.
-- dependent destruction H. eapply IHlts with c. assumption. reflexivity.
-- dependent destruction H. eapply IHlts with c. assumption. reflexivity.
-Qed.
-
-Lemma LTS_Respects_WD : forall p q α, Well_Defined_Input_in 0 p -> Well_Defined_Action α -> lts p α q 
-            ->  Well_Defined_Input_in 0 q.
-Proof.
-intros. revert H. revert H0. rename H1 into Transition. dependent induction Transition.
-* intros. dependent destruction H0.  apply WD_and_subst_rec. dependent destruction H. assumption.
-* intros. constructor.
-* intros. dependent destruction H. assumption.
-* intros. apply ForRecursionSanity. dependent destruction H. assumption. assumption.
-* intros. dependent destruction H1. assumption.
-* intros. dependent destruction H1. assumption.
-* intros. dependent destruction H. constructor. 
-  ** apply IHTransition1. assert (exists v', v = cst v'). eapply Output_are_good. exact H.
-     exact Transition1. destruct H2. subst. constructor. assumption.
-  ** apply IHTransition2. assert (exists v', v = cst v'). eapply Output_are_good. exact H.
-     exact Transition1. destruct H2. subst. constructor. assumption.
-* intros. dependent destruction H. constructor.
-  ** apply IHTransition2. assert (exists v', v = cst v'). eapply Output_are_good. exact H1.
-     exact Transition1. destruct H2. subst. constructor. assumption.
-  ** apply IHTransition1. assert (exists v', v = cst v'). eapply Output_are_good. exact H1.
-     exact Transition1. destruct H2. subst. constructor. assumption.
-* intros. dependent destruction H. constructor. apply IHTransition. assumption. assumption. assumption.
-* intros. dependent destruction H. constructor. assumption. apply IHTransition. assumption. assumption.
-* intros. dependent destruction H. apply IHTransition. assumption. assumption.
-* intros. dependent destruction H. apply IHTransition. assumption. assumption.
-Qed.
-
-
-(* Lemma to simplify the Data in Value for a transition *)
-Lemma OutputWithValue : forall p q a, lts p (ActOut a) q -> exists c d, a = c ⋉ d.
-Proof.
-intros. dependent destruction a. dependent induction H.
-- exists c. exists d. reflexivity.
-- destruct (IHlts c d). reflexivity. destruct H0. dependent destruction H0. exists x. exists x0. reflexivity.
-- destruct (IHlts c d). reflexivity. destruct H0. dependent destruction H0. exists x. exists x0. reflexivity.
-- destruct (IHlts c d). reflexivity. destruct H0. dependent destruction H0. exists x. exists x0. reflexivity.
-- destruct (IHlts c d). reflexivity. destruct H0. dependent destruction H0. exists x. exists x0. reflexivity.
-Qed.
-
-Lemma InputWithValue : forall p q a, lts p (ActIn a) q -> exists c v, a = c ⋉ v.
-Proof.
-intros. dependent destruction a. dependent induction H.
-- exists c. exists d. reflexivity.
-- destruct (IHlts c d). reflexivity. destruct H0. dependent destruction H0. exists x. exists x0. reflexivity.
-- destruct (IHlts c d). reflexivity. destruct H0. dependent destruction H0. exists x. exists x0. reflexivity.
-- destruct (IHlts c d). reflexivity. destruct H0. dependent destruction H0. exists x. exists x0. reflexivity.
-- destruct (IHlts c d). reflexivity. destruct H0. dependent destruction H0. exists x. exists x0. reflexivity.
-Qed.
-
-
-(* Peter Selinger Axioms (OutBuffered Agent with FeedBack) up to structural equivalence*)
-
-Lemma OBA_with_FB_First_Axiom : forall p q r a α,
-  lts p (ActOut a) q -> lts q α r ->
-  (exists r', lts p α r' /\ lts_then_sc r' (ActOut a) r). (* output-commutativity *)
-Proof.
-intros. assert (lts p (ActOut a) q). assumption. apply OutputWithValue in H1.
-decompose record H1. subst. eapply TransitionShapeForOutputSimplified in H.
-eapply lts_parR in H0. instantiate (1 := (x ! x0 • 𝟘)) in H0.
-edestruct (Congruence_Respects_Transition p ((x ! x0 • 𝟘) ‖ r) α).
-exists ((x ! x0 • 𝟘) ‖ q). split; assumption. destruct H2.
-assert (lts ((x ! x0 • 𝟘) ‖ r) (ActOut (x ⋉ x0)) (𝟘 ‖ r)). constructor. constructor.
-edestruct (Congruence_Respects_Transition x1 (𝟘 ‖ r) (ActOut (x ⋉ x0))).
-exists ((x ! x0 • 𝟘) ‖ r). split ; assumption. destruct H5.
-assert (x2 ≡* r). eauto with cgr.
-exists x1. split. assumption. exists x2. split; assumption.
-Qed.
-
-Lemma OBA_with_FB_Second_Axiom : forall p q1 q2 a μ, 
-  μ ≠ (ActOut a) ->
-  lts p (ActOut a) q1 ->
-  lts p (ActExt μ) q2 ->
-  ∃ r : proc, lts q1 (ActExt μ) r ∧ lts_then_sc q2 (ActOut a) r. (* output-confluence  *)
-Proof.
-intros. assert (lts p (ActOut a) q1). assumption. apply OutputWithValue in H2.
-decompose record H2. subst. rename x into c. rename x0 into v.
-eapply TransitionShapeForOutputSimplified in H0.
-edestruct (Congruence_Respects_Transition ((c ! v • 𝟘) ‖ q1) q2 μ).
-exists p. split. symmetry. assumption. assumption.
-destruct H3. inversion H3; subst.
-inversion H9. subst. now destruct H. 
-exists q3. split. assumption.
-assert (lts ((c ! v • 𝟘) ‖ q3) (ActOut (c ⋉ v)) (𝟘 ‖ q3)). constructor. constructor.
-edestruct (Congruence_Respects_Transition q2 (𝟘 ‖ q3) (ActOut (c ⋉ v))).
-exists ((c ! v • 𝟘) ‖ q3). split. eauto with cgr. assumption. destruct H6. exists x. split. assumption.
-eauto with cgr.
-Qed.
-
-Lemma OBA_with_FB_Third_Axiom : forall p1 p2 p3 a, 
-            lts p1 (ActOut a) p2 → lts p1 (ActOut a) p3 -> p2 ≡* p3. (* output-determinacy *)
-Proof.
-intros. assert (lts p1 (ActOut a) p2). assumption. apply OutputWithValue in H1.
-decompose record H1. subst. rename x into c. rename x0 into v.
-revert H0. revert p3. dependent induction H.
-- intros. inversion H0. subst. eauto with cgr.
-- intros. inversion H0;subst. 
-  * apply cgr_fullpar. eapply IHlts. eauto. eauto. assumption. eauto with cgr.
-  * apply TransitionShapeForOutputSimplified in H.
-    apply TransitionShapeForOutputSimplified in H6.
-    apply transitivity with (p2 ‖ ((c ! v • 𝟘) ‖ q2)). eauto with cgr. 
-    apply transitivity with ((p2 ‖ (c ! v • 𝟘)) ‖ q2). eauto with cgr. apply cgr_par.
-    eauto with cgr.
-- intros. inversion H0 ; subst.
-  * apply TransitionShapeForOutputSimplified in H.
-    apply TransitionShapeForOutputSimplified in H6.
-    apply transitivity with (((c ! v • 𝟘) ‖ p2) ‖ q2). eauto with cgr.
-    apply transitivity with (( p2 ‖ (c ! v • 𝟘)) ‖ q2). eauto with cgr.
-    apply transitivity with ( p2 ‖ ((c ! v • 𝟘) ‖ q2)). eauto with cgr. apply cgr_fullpar. reflexivity.
-    eauto with cgr.
-  * apply cgr_fullpar. reflexivity. eapply IHlts. eauto. eauto. assumption.
-- intros. exfalso. eapply guarded_does_no_output. eassumption.
-- intros. exfalso. eapply guarded_does_no_output. eassumption.
-Qed.
-
-Lemma OBA_with_FB_Fourth_Axiom : forall p1 p2 p3 a, lts p1 (ActOut a) p2 -> lts p2 (ActIn a) p3 
-                              -> lts_then_sc p1 τ p3. (* feedback *)
-Proof.
-intros. assert (lts p1 (ActOut a) p2). assumption. apply OutputWithValue in H1.
-decompose record H1. subst. rename x into c. rename x0 into v.
-eapply TransitionShapeForOutputSimplified in H.
-assert (lts (c ! v • 𝟘) (ActOut (c ⋉ v)) 𝟘). constructor.
-assert (lts ((c ! v • 𝟘) ‖ p2) τ  (𝟘 ‖ p3)). econstructor; eassumption.
-edestruct (Congruence_Respects_Transition p1 (𝟘 ‖ p3) τ). exists ((c ! v • 𝟘) ‖ p2).
-split; assumption. destruct H4. exists x. split. assumption. eauto with cgr.
-Qed.
-
-Lemma OBA_with_FB_Fifth_Axiom : forall p q1 q2 a,
-  lts p (ActOut a) q1 -> lts p τ q2 ->
-  (∃ q : proc, lts q1 τ q /\ lts_then_sc q2 (ActOut a) q) \/ lts_then_sc q1 (ActIn a) q2. (* output-tau  *)
-Proof.
-intros. assert (lts p (ActOut a) q1). assumption. apply OutputWithValue in H1.
-decompose record H1. subst. rename x into c. rename x0 into v.
-eapply TransitionShapeForOutputSimplified in H.
-edestruct (Congruence_Respects_Transition ((c ! v • 𝟘) ‖ q1) q2 τ). exists p. split. eauto with cgr. assumption.
-destruct H2. dependent induction H2.
-- inversion H2_; subst. right. exists q0. split. assumption. eauto with cgr. 
-- inversion H2_0.
-- inversion H2.
-- left. exists q0. split. assumption. 
-  assert (lts ((c ! v • 𝟘) ‖ q0) (ActOut (c ⋉ v)) (𝟘 ‖ q0)). constructor. constructor.
-  edestruct (Congruence_Respects_Transition q2 (𝟘 ‖ q0) (ActOut (c ⋉ v))). exists ((c ! v • 𝟘) ‖ q0).
-  split. eauto with cgr. assumption. destruct H5. exists x. split. assumption. eauto with cgr.
-Qed.
-
-
-Lemma ExtraAxiom : forall p1 p2 q1 q2 a,
-      lts p1 (ActOut a) q1 -> lts p2 (ActOut a) q2 -> q1 ≡* q2 -> p1 ≡* p2.
-Proof.
-intros. assert (lts p1 (ActOut a) q1). assumption. apply OutputWithValue in H2.
-decompose record H2. subst. rename x into c. rename x0 into v.
-eapply TransitionShapeForOutputSimplified in H0.
-eapply TransitionShapeForOutputSimplified in H.
-apply transitivity with ((c ! v • 𝟘) ‖ q1). assumption.
-apply transitivity with ((c ! v • 𝟘) ‖ q2). eauto with cgr. eauto with cgr.
-Qed. 
-
-Lemma Data_dec : forall (x y : Data) , {x = y} + {x <> y}.
-Proof.
-decide equality. 
-* destruct (decide(v = v0)). left. assumption. right. assumption.
-* destruct (decide (n = n0)). left. assumption. right. assumption.
-Qed.
-
-#[global] Instance data_eqdecision : EqDecision Data. by exact Data_dec . Defined.
-
-Definition encode_data (D : Data) : gen_tree (nat + Value) :=
-match D with
-  | cst v => GenLeaf (inr v)
-  | bvar i => GenLeaf (inl i)
-end.
-
-Definition decode_data (tree : gen_tree (nat + Value)) : Data :=
-match tree with
-  | GenLeaf (inr v) => cst v
-  | GenLeaf (inl i) => bvar i
-  | _ => bvar 0
-end.
-
-Lemma encode_decide_datas d : decode_data (encode_data d) = d.
-Proof. case d. 
-* intros. simpl. reflexivity.
-* intros. simpl. reflexivity.
-Qed.
-
-#[global] Instance data_countable : Countable Data.
-Proof.
-  refine (inj_countable' encode_data decode_data _).
-  apply encode_decide_datas.
-Qed.
-
-
-Fixpoint encode_equation (E : Equation Data) : gen_tree (nat + Data) :=
-match E with
-  | tt => GenLeaf (inl 1)
-  | ff => GenLeaf (inl 0)
-  | D1 ⩽ D2 => GenNode 2 [GenLeaf (inr D1) ; GenLeaf (inr D2)]
-  | e1 ∨ e2 => GenNode 3 [encode_equation e1 ; encode_equation e2]
-  | non e => GenNode 4 [encode_equation e] 
-end.
-
-Fixpoint decode_equation (tree : gen_tree (nat + Data)) : Equation Data :=
-match tree with
-  | GenLeaf (inl 1) => tt
-  | GenLeaf (inl 0) => ff
-  | GenNode 2 [GenLeaf (inr d); GenLeaf (inr d')] => d ⩽ d'
-  | GenNode 3 [p ; q] => (decode_equation p) ∨ (decode_equation q)
-  | GenNode 4 [t'] => non (decode_equation t')
-  | _ => ff
-end. 
-
-Lemma Equation_dec : forall (x y : Equation Data) , {x = y} + {x <> y}.
-Proof.
-decide equality. apply Data_dec. apply Data_dec.
-Qed.
-
-#[global] Instance equation_dec : EqDecision (Equation Data). exact Equation_dec. Defined.
-
-Lemma encode_decide_equations p : decode_equation (encode_equation p) = p.
-Proof. 
-induction p.
-* simpl. reflexivity.
-* simpl. reflexivity.
-* simpl. reflexivity.
-* simpl. rewrite IHp1. rewrite IHp2. reflexivity.
-* simpl. rewrite IHp. reflexivity.
-Qed.
-
-#[global] Instance equation_countable : Countable (Equation Data).
-Proof.
-  refine (inj_countable' encode_equation decode_equation _).
-  apply encode_decide_equations.
-Qed.
-
-Lemma TypeOfActions_dec : forall (x y : TypeOfActions) , {x = y} + {x <> y}.
-Proof.
-decide equality. 
-* destruct (decide(d = d0)). left. assumption. right. assumption.
-* destruct (decide (c = c0)). left. assumption. right. assumption.
-Qed.
-
-#[global] Instance TypeOfActions_eqdecision : EqDecision TypeOfActions. by exact TypeOfActions_dec . Defined.
-
-Fixpoint proc_dec (x y : proc) : { x = y } + { x <> y }
-with gproc_dec (x y : gproc) : { x = y } + { x <> y }.
-Proof.
-decide equality. 
-* destruct (decide(n = n0));eauto.
-* destruct (decide(n = n0));eauto.
-* destruct (decide(e = e0));eauto. 
-* destruct (decide(d = d0));eauto.
-* destruct (decide(c = c0));eauto.
-* decide equality. destruct (decide(c = c0));eauto.
-Qed.
-
-#[global] Instance proc_eqdecision : EqDecision proc. by exact proc_dec. Defined.
-
-Definition encode_TypeOfActions (a : TypeOfActions) : gen_tree (nat + (Channel + Data)) :=
-match a with
-  | act c v => GenNode 0 [GenLeaf (inr (inl c)) ; GenLeaf (inr (inr v))]
-end.
-
-Definition decode_TypeOfActions (tree :gen_tree (nat + (Channel + Data))) : option TypeOfActions :=
-match tree with
-  | GenNode 0 [GenLeaf (inr (inl c)); GenLeaf (inr (inr v))] => Some (act c v)
-  | _ => None
-end.
-
-Lemma encode_decide_TypeOfActions p : decode_TypeOfActions (encode_TypeOfActions  p) = Some p.
-Proof. 
-induction p. 
-* simpl. reflexivity.
-Qed.
-
-#[global] Instance TypeOfActions_countable : Countable TypeOfActions.
-Proof.
-  eapply inj_countable with encode_TypeOfActions decode_TypeOfActions. 
-  intro. apply encode_decide_TypeOfActions.
-Qed.
-
-Fixpoint encode_proc (p: proc) : gen_tree (nat + (((Equation Data ) + TypeOfActions) + Channel)) :=
-  match p with
-  | p ‖ q  => GenNode 0 [encode_proc p; encode_proc q]
-  | c ! v • 𝟘  => GenLeaf (inr $ inl $ inr $ (c ⋉ v))
-  | pr_var i => GenNode 2 [GenLeaf $ inl i]
-  | rec x • P => GenNode 3 [GenLeaf $ inl x; encode_proc P]
-  | If C Then A Else B => GenNode 4 [GenLeaf (inr ( inl (inl C))) ; encode_proc A; encode_proc B]
-  | g gp => GenNode 1 [encode_gproc gp]
-  end
-with
-encode_gproc (gp: gproc) : gen_tree (nat + (((Equation Data ) + TypeOfActions) + Channel)) :=
-  match gp with
-  | ① => GenNode 1 []
-  | 𝟘 => GenNode 0 []
-  | c ? p => GenNode 2 [GenLeaf (inr $ inr c); encode_proc p]
-  | t • p => GenNode 3 [encode_proc p]
-  | gp + gq => GenNode 4 [encode_gproc gp; encode_gproc gq]
-  end.
-  
-Definition Channel_of (a : TypeOfActions) : Channel := 
-match a with 
-| act c d => c
-end.
-
-Definition Data_of (a : TypeOfActions) : Data := 
-match a with 
-| act c d => d
-end.
-
-Fixpoint decode_proc (t': gen_tree (nat + (((Equation Data ) + TypeOfActions) + Channel))) : proc :=
-  match t' with
-  | GenNode 0 [ep; eq] => (decode_proc ep) ‖ (decode_proc eq)
-  | GenLeaf (inr ( inl (inr a))) => (Channel_of a) ! (Data_of a) • 𝟘
-  | GenNode 2 [GenLeaf (inl i)] => pr_var i
-  | GenNode 3 [GenLeaf (inl i); egq] => rec i • (decode_proc egq)
-  | GenNode 4 [GenLeaf (inr ( inl (inl C))); A; B] => If C Then (decode_proc A) Else (decode_proc B)
-  | GenNode 1 [egp] => g (decode_gproc egp)
-  | _ => ① 
-  end
-with
-decode_gproc (t': gen_tree (nat + (((Equation Data ) + TypeOfActions) + Channel))): gproc :=
-  match t' with
-  | GenNode 1 [] => ①
-  | GenNode 0 [] => 𝟘
-  | GenNode 2 [GenLeaf (inr (inr c)); ep] => c ? (decode_proc ep)
-  | GenNode 3 [eq] => t • (decode_proc eq)
-  | GenNode 4 [egp; egq] => (decode_gproc egp) + (decode_gproc egq)
-  | _ => ① 
-  end.
-
-Lemma encode_decide_procs p : decode_proc (encode_proc p) = p
-with encode_decide_gprocs p : decode_gproc (encode_gproc p) = p.
-Proof. all: case p. 
-* intros. simpl. rewrite (encode_decide_procs p0). rewrite (encode_decide_procs p1). reflexivity.
-* intros. simpl. reflexivity.
-* intros. simpl. rewrite (encode_decide_procs p0). reflexivity.
-* intros. simpl. rewrite (encode_decide_procs p0). rewrite (encode_decide_procs p1). reflexivity.
-* intros. simpl. reflexivity.
-* intros. simpl. rewrite (encode_decide_gprocs g0). reflexivity.
-* intros. simpl. reflexivity. 
-* intros. simpl. reflexivity. 
-* intros. simpl. rewrite (encode_decide_procs p0). reflexivity.
-* intros. simpl. rewrite (encode_decide_procs p0). reflexivity.
-* intros. simpl. rewrite (encode_decide_gprocs g0). rewrite (encode_decide_gprocs g1). reflexivity.
-Qed.
-
-#[global] Instance proc_count : Countable proc.
-refine (inj_countable' encode_proc decode_proc _).
-  apply encode_decide_procs.
-Qed.
-#[global] Instance Singletons_of_TypeOfActions : SingletonMS TypeOfActions (gmultiset TypeOfActions) 
-:=gmultiset_singleton.
-#[global] Instance Singletons_of_proc : Singleton proc (gset proc) := gset_singleton.
-#[global] Instance Empty_of_proc : Empty (gset proc) := gset_empty.
-#[global] Instance Union_of_proc : Union (gset proc) := gset_union.
-#[global] Instance SemiSet_of_proc : SemiSet proc (gset proc) := gset_semi_set.
-
-(* Next Obligations *)
-Fixpoint moutputs_of p : gmultiset TypeOfActions := 
-match p with
-  | P ‖ Q => (moutputs_of P) ⊎ (moutputs_of Q)
-  | pr_var _ => ∅
-  | rec _ • _ => ∅
-  | If C Then P Else Q => ∅
-  | c ! v • 𝟘 => {[+ c ⋉ v +]}
-  | g _ => ∅
-end.  
-Definition outputs_of p := dom (moutputs_of p).
-
-Lemma mo_equiv_spec_step : forall {p q}, p ≡ q -> moutputs_of p = moutputs_of q.
-Proof. intros. dependent induction H; multiset_solver. Qed.
-
-Lemma mo_equiv_spec : forall {p q}, p ≡* q -> moutputs_of p = moutputs_of q.
-Proof.
-  intros p q hcgr.
-  induction hcgr. now eapply mo_equiv_spec_step.
-  etrans; eauto.
-Qed.
-
-Lemma mo_spec p a q : lts p (ActOut a) q -> moutputs_of p = {[+ a +]} ⊎ moutputs_of q.
-Proof.
-  intros l. assert (lts p (ActOut a) q). assumption. apply OutputWithValue in H.
-  decompose record H. subst. rename x into c. rename x0 into v.
-  eapply TransitionShapeForOutputSimplified, mo_equiv_spec in l. simpl in l. eauto.
-Qed.
-
-Lemma mo_spec_l e a :
-  a ∈ moutputs_of e -> {e' | lts e (ActExt $ ActOut a) e' /\ moutputs_of e' = moutputs_of e ∖ {[+ a +]}}.
-Proof.
-  intros mem.
-  dependent induction e.
-  + cbn in mem.
-    destruct (decide (a ∈ moutputs_of e1)).
-    destruct (IHe1 a e) as (e1' & lts__e1 & eq).
-    exists (pr_par e1' e2). repeat split; eauto with ccs.
-    multiset_solver.
-    destruct (decide (a ∈ moutputs_of e2)).
-    destruct (IHe2 a e) as (e2' & lts__e2 & eq).
-    exists (pr_par e1 e2'). repeat split; eauto with ccs.
-    multiset_solver.
-    contradict mem. intro mem. multiset_solver.
-    + exfalso. multiset_solver.
-    + exfalso. multiset_solver.
-    + exfalso. multiset_solver.
-  + exists (g 𝟘).
-    assert (a = c ⋉ d). multiset_solver. subst.
-    repeat split; eauto with ccs. multiset_solver.
-  + simpl in mem. exfalso. set_solver. 
-Qed.
-
-Lemma mo_spec_r e a :
-  {e' | lts e (ActExt $ ActOut a) e' /\ moutputs_of e' = moutputs_of e ∖ {[+ a +]}} -> a ∈ moutputs_of e.
-Proof.
-  dependent induction e; intros (e' & l & mem).
-  + cbn.
-    inversion l; subst.
-    eapply gmultiset_elem_of_disj_union. left.
-    eapply IHe1. exists p2. split.
-    eassumption. cbn in mem. multiset_solver.
-    eapply gmultiset_elem_of_disj_union. right.
-    eapply IHe2. exists q2. split.
-    eassumption. cbn in mem. multiset_solver.
-  + inversion l.
-  + inversion l.
-  + inversion l.    
-  + inversion l; subst. set_solver.
-  + destruct a. now eapply guarded_does_no_output in l.
-Qed.
-
-
-Lemma outputs_of_spec2 p a : a ∈ outputs_of p -> {q | lts p (ActExt (ActOut a)) q}.
-Proof.
-  intros mem.
-  eapply gmultiset_elem_of_dom in mem.
-  eapply mo_spec_l in mem.
-  firstorder.
-Qed.
-
-Lemma outputs_of_spec1_zero (p : proc) (a : TypeOfActions) : {q | lts p (ActExt (ActOut a)) q} 
-      -> a ∈ outputs_of p.
-Proof.    
-  intros (p' & lts__p).
-  dependent induction p.
-  + eapply gmultiset_elem_of_dom.
-    cbn. inversion lts__p; subst. apply IHp1 in H3. eapply gmultiset_elem_of_dom in H3. multiset_solver.
-     apply IHp2 in H3. eapply gmultiset_elem_of_dom in H3. multiset_solver.
-  + inversion lts__p; subst.
-  + inversion lts__p; subst.
-  + inversion lts__p; subst.
-  + inversion lts__p; subst. unfold outputs_of. multiset_solver.
-  + assert (lts g0 (ActOut a) p'). assumption. apply OutputWithValue in H.
-    decompose record H. subst. rename x into c. rename x0 into v.
-    now eapply guarded_does_no_output in lts__p.
-Qed.
-
-Lemma outputs_of_spec1 (p : proc) (a : TypeOfActions) (q : proc) : lts p (ActExt (ActOut a)) q
-      -> a ∈ outputs_of p.
-Proof.
-intros. eapply outputs_of_spec1_zero. exists q. assumption.
-Qed.
-
-Fixpoint lts_set_output (p : proc) (a : TypeOfActions) : gset proc:=
-match p with
-  | p1 ‖ p2 => 
-      let ps1 := lts_set_output p1 a in
-      let ps2 := lts_set_output p2 a in
-      (* fixme: find a way to map over sets. *)
-      list_to_set (map (fun p => p ‖ p2) (elements ps1)) ∪ list_to_set (map (fun p => p1 ‖ p) (elements ps2))
-  | pr_var _ => ∅
-  | rec _ • _ => ∅
-  | If _ Then _ Else _ => ∅
-  | c ! v • 𝟘 => if decide(a = (c ⋉ v)) then {[ (g 𝟘) ]} else ∅
-  | g _  => ∅
-end.
-
-Fixpoint lts_set_input_g (g : gproc) (a : TypeOfActions) : gset proc :=
-  match g with
-  | c ? p => if decide(Channel_of a = c) then {[ p^(Data_of a) ]} else ∅
-  | g1 + g2 => lts_set_input_g g1 a ∪ lts_set_input_g g2 a
-  | ① => ∅
-  | 𝟘 => ∅
-  | t • p => ∅
-  end.
-  
-Fixpoint lts_set_input (p : proc) (a : TypeOfActions) : gset proc :=
-match p with
-  | p1 ‖ p2 =>
-      let ps1 := lts_set_input p1 a in
-      let ps2 := lts_set_input p2 a in
-      list_to_set (map (fun p => p ‖ p2) (elements ps1)) ∪ list_to_set (map (fun p => p1 ‖ p) (elements ps2))
-  | pr_var _ => ∅
-  | rec _ • _ => ∅ 
-  | c ! v • 𝟘 => ∅
-  | If _ Then _ Else _ => ∅
-  | g gp => lts_set_input_g gp a  
-  end.
-  
-Fixpoint lts_set_tau_g (gp : gproc) : gset proc :=
-match gp with
-  | c ? p => ∅
-  | ① => ∅
-  | 𝟘 => ∅
-  | t • p => {[ p ]}
-  | gp1 + gp2 => lts_set_tau_g gp1 ∪ lts_set_tau_g gp2
-end.
-
-
-
-Fixpoint lts_set_tau (p : proc) : gset proc :=
-match p with
-  | p1 ‖ p2 =>
-      let ps1_tau : gset proc := list_to_set (map (fun p => p ‖ p2) (elements $ lts_set_tau p1)) in
-      let ps2_tau : gset proc := list_to_set (map (fun p => p1 ‖ p) (elements $ lts_set_tau p2)) in
-      let ps_tau := ps1_tau ∪ ps2_tau in
-      let acts1 := outputs_of p1 in
-      let acts2 := outputs_of p2 in
-      let ps1 :=
-        flat_map (fun a =>
-                    map
-                      (fun '(p1 , p2) => p1 ‖ p2)
-                      (list_prod (elements $ lts_set_output p1 a) (elements $ lts_set_input p2 a)))
-        (elements $ outputs_of p1) in
-      let ps2 :=
-        flat_map
-          (fun a =>
-             map
-               (fun '(p1 , p2) => p1 ‖ p2)
-               (list_prod (elements $ lts_set_input p1 a) (elements $ lts_set_output p2 a)))
-          (elements $ outputs_of p2)
-      in
-      ps_tau ∪ list_to_set ps1 ∪ list_to_set ps2
-  | c ! v • 𝟘 => ∅
-  | pr_var _ => ∅
-  | rec x • p => {[ pr_subst x p (rec x • p) ]}
-  | If C Then A Else B => match (Eval_Eq C) with 
-                          | Some true => {[ A ]}
-                          | Some false => {[ B ]}
-                          | None => ∅
-                          end
-  | g gp => lts_set_tau_g gp
-end.
-
-Lemma lts_set_output_spec0 p a q : q ∈ lts_set_output p a -> lts p (ActExt (ActOut a)) q.
-Proof.
-  intro mem.
-  dependent induction p; simpl in mem; try now inversion mem.
-  - eapply elem_of_union in mem as [mem | mem]. 
-    * eapply elem_of_list_to_set, elem_of_list_fmap in mem as (q' & eq & mem). subst.
-    apply lts_parL. apply IHp1. rewrite elem_of_elements in mem. set_solver.
-    * eapply elem_of_list_to_set, elem_of_list_fmap in mem as (q' & eq & mem). subst.
-    apply lts_parR. apply IHp2. rewrite elem_of_elements in mem. exact mem.
-  -  case (TypeOfActions_dec a (c ⋉ d)) in mem.
-    + rewrite e. rewrite e in mem.
-      destruct (decide (c ⋉ d = c ⋉ d)). subst. assert (q = (g 𝟘)). set_solver.
-      rewrite H. apply lts_output. exfalso. set_solver.
-    + destruct (decide (a = c ⋉ d)). exfalso. apply n. assumption. set_solver.
-Qed.
-
-Lemma lts_set_output_spec1 p a q : lts p (ActExt $ ActOut a) q -> q ∈ lts_set_output p a.
-Proof.
-  intro l. dependent induction l; try set_solver.
-  simpl. destruct (decide (c ⋉ v = c ⋉ v)). set_solver. exfalso. apply n. reflexivity.
-Qed.
-
-Lemma lts_set_input_spec0 p a q : q ∈ lts_set_input p a -> lts p (ActExt $ ActIn a) q.
-Proof.
-  intro mem.
-  dependent induction p; simpl in mem; try set_solver.
-  + eapply elem_of_union in mem. destruct mem.
-    ++ eapply elem_of_list_to_set in H.
-       eapply elem_of_list_fmap in H as (q' & eq & mem). subst.
-       rewrite elem_of_elements in mem. eauto with ccs.
-    ++ eapply elem_of_list_to_set in H.
-       eapply elem_of_list_fmap in H as (q' & eq & mem). subst.
-       rewrite elem_of_elements in mem. eauto with ccs.
-  + dependent induction g0; simpl in mem; try set_solver.
-      ++ destruct (decide (Channel_of a = c)).
-         +++ subst. eapply elem_of_singleton_1 in mem. subst. destruct a. simpl. apply lts_input.
-         +++ destruct a. simpl in *. inversion mem.
-      ++ eapply elem_of_union in mem. destruct mem; eauto with ccs.
-Qed.
-
-Lemma lts_set_input_spec1 p a q : lts p (ActExt $ ActIn a) q -> q ∈ lts_set_input p a.
-Proof.
-  intro l. dependent induction l; try set_solver.
-  simpl. destruct (decide (c = c)). set_solver. exfalso. apply n. reflexivity.
-Qed.
-
-
-Lemma lts_set_tau_spec0 p q : q ∈ lts_set_tau p -> lts p τ q.
-Proof.
-  - intro mem.
-    dependent induction p; simpl in mem.
-    + eapply elem_of_union in mem. destruct mem as [mem1 | mem2].
-      ++ eapply elem_of_union in mem1.
-         destruct mem1.
-         eapply elem_of_union in H as [mem1 | mem2]. 
-         eapply elem_of_list_to_set, elem_of_list_fmap in mem1 as (t' & eq & h); subst.
-         rewrite elem_of_elements in h. eauto with ccs.
-         eapply elem_of_list_to_set, elem_of_list_fmap in mem2 as (t' & eq & h); subst.
-         rewrite elem_of_elements in h. eauto with ccs.
-         eapply elem_of_list_to_set, elem_of_list_In, in_flat_map in H as (t' & eq & h); subst.
-         eapply elem_of_list_In, elem_of_list_fmap in h as ((t1 & t2) & eq' & h'). subst.
-         eapply elem_of_list_In, in_prod_iff in h' as (mem1 & mem2).
-         eapply elem_of_list_In in mem1. rewrite elem_of_elements in mem1.
-         eapply elem_of_list_In in mem2. rewrite elem_of_elements in mem2.
-         eapply lts_set_output_spec0 in mem1.
-         eapply lts_set_input_spec0 in mem2. destruct t'. eapply lts_comL. exact mem1. exact mem2.
-      ++ eapply elem_of_list_to_set, elem_of_list_In, in_flat_map in mem2 as (t' & eq & h); subst.
-         eapply elem_of_list_In, elem_of_list_fmap in h as ((t1 & t2) & eq' & h'). subst.
-         eapply elem_of_list_In, in_prod_iff in h' as (mem1 & mem2).
-         eapply elem_of_list_In in mem1. rewrite elem_of_elements in mem1.
-         eapply elem_of_list_In in mem2. rewrite elem_of_elements in mem2.
-         eapply lts_set_input_spec0 in mem1.
-         eapply lts_set_output_spec0 in mem2. destruct t'. eapply lts_comR. exact mem2. exact mem1.
-    + inversion mem.
-    + eapply elem_of_singleton_1 in mem. subst; eauto with ccs.
-    + destruct (decide (Eval_Eq e = Some true)).
-      * rewrite e0 in mem. assert (q = p1). set_solver. rewrite H. constructor. assumption.
-      * destruct (decide (Eval_Eq e = Some false)). rewrite e0 in mem. 
-        assert (q = p2). set_solver. rewrite H. constructor. assumption.
-        assert (Eval_Eq e = None). destruct (Eval_Eq e). destruct b. exfalso. apply n. reflexivity.
-        exfalso. apply n0. reflexivity. reflexivity. rewrite H in mem. set_solver.
-    + inversion mem.
-    + dependent induction g0; simpl in mem; try set_solver;
-        try eapply elem_of_singleton_1 in mem; subst; eauto with ccs.
-      eapply elem_of_union in mem as [mem1 | mem2]; eauto with ccs.
-Qed.
-
-Lemma lts_set_tau_spec1 p q : lts p τ q -> q ∈ lts_set_tau p.
-Proof. 
-  intro l. dependent induction l; simpl; try set_solver.
-  - rewrite H. set_solver. 
-  - rewrite H. set_solver. 
-  - eapply elem_of_union. left.
-    eapply elem_of_union. right.
-    eapply elem_of_list_to_set.
-    rewrite elem_of_list_In. rewrite in_flat_map.
-    exists (c ⋉ v). split.
-    + eapply elem_of_list_In, elem_of_elements.
-      eapply outputs_of_spec1_zero. eauto.
-    + eapply elem_of_list_In, elem_of_list_fmap.
-      exists (p2 , q2). split.
-      ++ reflexivity.
-      ++ eapply elem_of_list_In, in_prod_iff; split; eapply elem_of_list_In, elem_of_elements.
-         eapply lts_set_output_spec1; eauto with ccs.
-         eapply lts_set_input_spec1; eauto with ccs.
-  - eapply elem_of_union. right.
-    eapply elem_of_list_to_set.
-    rewrite elem_of_list_In. rewrite in_flat_map.
-    exists (c ⋉ v). split.
-    + eapply elem_of_list_In, elem_of_elements.
-      eapply outputs_of_spec1_zero. exists p2. exact l1.
-    + eapply elem_of_list_In, elem_of_list_fmap.
-      exists (q2 , p2). split.
-      ++ reflexivity.
-      ++ eapply elem_of_list_In, in_prod_iff; split; eapply elem_of_list_In, elem_of_elements.
-         eapply lts_set_input_spec1; eauto with ccs.
-         eapply lts_set_output_spec1; eauto with ccs.
-Qed.
-
-
-Definition lts_set (p : proc) (α : Act TypeOfActions): gset proc :=
-  match α with
-  | τ => lts_set_tau p
-  | ActExt (ActIn a) => lts_set_input p a
-  | ActExt (ActOut a) => lts_set_output p a
-  end.
-
-Lemma lts_set_spec0 p α q : q ∈ lts_set p α -> lts p α q.
-Proof.
-  destruct α as [[a|a]|].
-  - now eapply lts_set_input_spec0.
-  - now eapply lts_set_output_spec0.
-  - now eapply lts_set_tau_spec0.
-Qed.
-
-Lemma lts_set_spec1 p α q : lts p α q -> q ∈ lts_set p α.
-Proof.
-  destruct α as [[a|a]|].
-  - now eapply lts_set_input_spec1.
-  - now eapply lts_set_output_spec1.
-  - now eapply lts_set_tau_spec1.
-Qed.
-
-Definition proc_stable p α := lts_set p α = ∅.
-
-Lemma lts_dec p α q : { lts p α q } + { ~ lts p α q }.
-Proof.
-  destruct (decide (q ∈ lts_set p α)).
-  - eapply lts_set_spec0 in e. eauto.
-  - right. intro l. now eapply lts_set_spec1 in l.
-Qed.
-
-Lemma proc_stable_dec p α : Decision (proc_stable p α).
-Proof. destruct (decide (lts_set p α = ∅)); [ left | right ]; eauto. Qed.
-
-Lemma gset_nempty_ex (g : gset proc) : g ≠ ∅ -> {p | p ∈ g}.
-Proof.
-  intro n. destruct (elements g) eqn:eq.
-  + destruct n. eapply elements_empty_iff in eq. set_solver.
-  + exists p. eapply elem_of_elements. rewrite eq. set_solver.
-Qed.
-
-(* Making VACCS Instance of each class *)
-
-#[global] Program Instance VACCS_Label : Label TypeOfActions := 
-  {| label_eqdec := TypeOfActions_dec ;
-  label_countable := TypeOfActions_countable |}. (* useless, already said it, it is just a reminder *)
-
-#[global] Program Instance VACCS_Lts : Lts proc TypeOfActions := 
-  {| lts_step x ℓ y  := lts x ℓ y ;
-     lts_state_eqdec := proc_dec ;
-     lts_step_decidable p α q := lts_dec p α q ;
-     lts_outputs := outputs_of ;
-     lts_outputs_spec1 p1 x p2 := outputs_of_spec1 p1 x p2;
-     lts_outputs_spec2 p1 x := outputs_of_spec2 p1 x;
-     lts_stable p := proc_stable p;
-     lts_stable_decidable p α := proc_stable_dec p α 
-    |}.
-    Next Obligation.
-        intros p [[a|a]|]; intro hs;eapply gset_nempty_ex in hs as (r & l); eapply lts_set_spec0 in l; 
-        exists r; assumption.
-    Qed.
-    Next Obligation.  
-        intros p [[a|a]|]; intros (q & mem); intro eq; eapply lts_set_spec1 in mem; set_solver.
-    Qed.
-
-#[global] Program Instance VACCS_LtsEq : LtsEq proc TypeOfActions := 
-  {| eq_rel x y  := cgr x y;
-     eq_rel_refl p := cgr_refl p;
-     eq_symm p q := cgr_symm p q;
-     eq_trans x y z:= cgr_trans x y z;
-     eq_spec p q α := Congruence_Respects_Transition p q α |}.
-
-#[global] Program Instance VACCS_LtsOba : LtsOba proc TypeOfActions :=
-  {| lts_oba_output_commutativity p q r a α := OBA_with_FB_First_Axiom p q r a α;
-     lts_oba_output_confluence p q1 q2 a μ := OBA_with_FB_Second_Axiom p q1 q2 a μ;
-     lts_oba_output_deter p1 p2 p3 a := OBA_with_FB_Third_Axiom p1 p2 p3 a;
-     lts_oba_output_tau p q1 q2 a := OBA_with_FB_Fifth_Axiom p q1 q2 a;
-     lts_oba_output_deter_inv p1 p2 q1 q2 a := ExtraAxiom p1 p2 q1 q2 a;
-     lts_oba_mo p := moutputs_of p 
-  |}.
-  Next Obligation.
-    intros. simpl. unfold outputs_of.
-    now rewrite gmultiset_elem_of_dom.
-  Qed.
-  Next Obligation.
-    intros. simpl. unfold outputs_of.
-    now eapply mo_spec.
-  Qed.
-  
-
-#[global] Program Instance VACCS_LtsObaFB : LtsObaFB proc TypeOfActions :=
-  {| lts_oba_fb_feedback p1 p2 p3 a := OBA_with_FB_Fourth_Axiom p1 p2 p3 a |}.
-
-*)
-
-(* Definition test_term :=  (ν ν (1 ! 0 • (0 ? 𝟘) + 𝟘) ‖ 0 ? (0 ! 3 • 𝟘) + 𝟘).
-
-Lemma test_term_sts: sts test_term (ν ν (0 ? 𝟘 ‖ 0 ! 3 • 𝟘)).
-Proof.
-unfold test_term.
-eapply sts_res.
-eapply sts_cong.
-- apply cgr_scope_rev.
-- eapply sts_res. eapply sts_com.
-- simpl. asimpl. apply cgr_refl.
-Qed.
-
-Lemma check : 
-  (@subst2 _ _ _ _ Subst_proc ids (@scons Data O ids)
-  (gpr_output 0 (@subst1 _ _ _ Subst_Data ids 4) 𝟘))= 
-0 ! 3 • 𝟘.
-Proof.
-reflexivity.
-Qed.
-
-Lemma test_term_lts: lts test_term τ
-  (ν ν (0 ? 𝟘 ‖ 0 ! 3 • 𝟘)).
-  (* (subst_proc ids (@scons Data (var_Data O) ids)
-  (gpr_output 0
-  (Subst_Data ids 4) (Subst_proc ids (@scons Data O ids) 𝟘)
-  )))). *)
-Proof.
-unfold test_term.
-unfold Subst_proc. Set Printing All.
-(* eexists. *)
-assert (τ = Shift_Action τ) by reflexivity. rewrite H.
-eapply lts_res.
-eapply (@lts_close_l 1).
-- eapply (@lts_open 1).
-  + intro F. inversion F.
-  + eapply lts_choiceL. eapply lts_output.
-- eapply lts_choiceL. rewrite <- check. apply lts_input.
-Set Printing All.
-Show Proof.
-Qed.
-
- *)
